Moved common lemmas to sequtils

inductive_proof/Append-only_log/App.fst
@@ -32,12 +32,6 @@ let eq_is_equiv (a b:concrete_st)
 // (the only operation is write a message)
 type app_op_t:eqtype = string
 
-let is_prefix_s (p l:concrete_st) : Tot prop =
-  Seq.length l >= Seq.length p /\ Seq.equal p (Seq.slice l 0 (Seq.length p))
-
-let is_suffix_s (s l:concrete_st) : Tot prop =
-  Seq.length l >= Seq.length s /\ Seq.equal s (Seq.slice l (Seq.length l - Seq.length s) (Seq.length l))
-
 // apply an operation to a state
 let do (s:concrete_st) (op:op_t) : concrete_st =
   cons (fst op, snd op) s 
@@ -50,9 +44,6 @@ let lem_do (a b:concrete_st) (op:op_t)
 let resolve_conflict (x:op_t) (y:op_t{fst x <> fst y}) : resolve_conflict_res =
   if lt (fst y) (fst x) then First_then_second else Second_then_first
 
-let mem_id_s (id:nat) (l:concrete_st) : bool =
-  mem_assoc_fst id l
-
 //#push-options "--z3rlimit 50"
 let rec union_s (l1 l2:concrete_st) 
   : Tot (u:concrete_st{forall e. mem e u <==> mem e l1 \/ mem e l2}) 
@@ -63,51 +54,38 @@ let rec union_s (l1 l2:concrete_st)
   |_, 0 -> l1
   |_, _ ->  if (fst (head l1) >= fst (head l2) )
              then (mem_cons (head l1) (union_s (tail l1) l2);
-                   //lemma_append_count_assoc_fst (create 1 (head l1)) (union_s (tail l1) l2);
                    cons (head l1) (union_s (tail l1) l2))
              else (mem_cons (head l2) (union_s l1 (tail l2));
-                   //lemma_append_count_assoc_fst (create 1 (head l2)) (union_s l1 (tail l2));
                    cons (head l2) (union_s l1 (tail l2)))
 
-let diff_s (s1:concrete_st) (lca:concrete_st{is_suffix_s lca s1}) 
-  : Tot (d:concrete_st{(s1 == Seq.append d lca) /\
-                       (forall id. mem_id_s id s1 <==> mem_id_s id d \/ mem_id_s id lca)}) =
-  let s = fst (split s1 (length s1 - length lca)) in
-  lemma_split s1 (length s1 - length lca);
-  lemma_mem_append s lca;
-  lemma_append_count_assoc_fst s lca;
-  s
-  
 let rec lem_foldl (s:concrete_st) (l:log)
   : Lemma (requires true)
           (ensures (length l = 0 ==> (apply_log s l = s)) /\
-                   (is_suffix_s s (apply_log s l)) /\
+                   (is_suffix s (apply_log s l)) /\
                    (length l > 0 ==> length (apply_log s l) > length s) /\
-                   (forall id. mem_id_s id (apply_log s l) <==> mem_id_s id s \/ mem_id id l))
+                   (forall id. mem_assoc_fst id (apply_log s l) <==> mem_assoc_fst id s \/ mem_id id l))
           (decreases length l)
-          [SMTPat (is_suffix_s s (apply_log s l))]
+          [SMTPat (is_suffix s (apply_log s l))]
   = match length l with
     |0 -> ()
-    //|1 -> ()
-    |_ -> assert (is_suffix_s s (do s (head l)));
+    |_ -> assert (is_suffix s (do s (head l)));
          lem_foldl (do s (head l)) (tail l)
 
 let lem_foldl_forall (s:concrete_st) 
-  : Lemma (ensures (forall l. (is_suffix_s s (apply_log s l)))) = ()
+  : Lemma (ensures (forall l. (is_suffix s (apply_log s l)))) = ()
 
 let concrete_merge (lca s1 s2:concrete_st) 
   : Pure concrete_st
          (requires (exists l1 l2. apply_log lca l1 == s1 /\ apply_log lca l2 == s2))
-         (ensures (fun _ -> True)) =
-  //lem_foldl_forall lca;
-  let la = diff_s s1 lca in
-  let lb = diff_s s2 lca in
+         (ensures (fun m -> (lca == s1 ==> m == s2) /\ (lca == s2 ==> m == s1))) =
+  let la = diff_suf s1 lca in
+  let lb = diff_suf s2 lca in
   let u = union_s la lb in 
   lemma_mem_append u lca;
   Seq.append u lca
 
 let rec lem_union_comm (l1 l2:concrete_st) 
-  : Lemma (requires (forall id. mem_id_s id l1 ==> not (mem_id_s id l2)))
+  : Lemma (requires (forall id. mem_assoc_fst id l1 ==> not (mem_assoc_fst id l2)))
           (ensures eq (union_s l1 l2) (union_s l2 l1)) 
           (decreases %[length l1; length l2]) =
   match length l1, length l2 with
@@ -120,60 +98,34 @@ let rec lem_union_comm (l1 l2:concrete_st)
              else (mem_cons (head l2) (union_s l1 (tail l2));
                    lem_union_comm l1 (tail l2))
 
-let unique_st (s:concrete_st) = distinct_assoc_fst s
-
 let do_is_unique (s:concrete_st) (op:op_t) 
-  : Lemma (requires unique_st s /\ (not (mem_id_s (fst op) s)))
-          (ensures unique_st (do s op) /\ length (do s op) = length s + 1) =
-  assert (unique_st s);
-  assert (unique_st (create 1 (fst op, snd op))); 
+  : Lemma (requires distinct_assoc_fst s /\ (not (mem_assoc_fst (fst op) s)))
+          (ensures distinct_assoc_fst (do s op) /\ length (do s op) = length s + 1) =
+  assert (distinct_assoc_fst s);
+  assert (distinct_assoc_fst (create 1 (fst op, snd op))); 
   distinct_append (create 1 (fst op, snd op)) s
 
-#push-options "--z3rlimit 50"
-let rec lem_foldl1 (s:concrete_st) (l:log)
-  : Lemma (requires unique_st s /\ distinct_ops l /\
-                    (forall id. mem_id_s id s ==> not (mem_id id l)))
-          (ensures unique_st (apply_log s l) /\ length (apply_log s l) = length s + length l)
+#push-options "--z3rlimit 100"
+let rec lem_foldl_uni (s:concrete_st) (l:log)
+  : Lemma (requires distinct_assoc_fst s /\ distinct_ops l /\
+                    (forall id. mem_assoc_fst id s ==> not (mem_id id l)))
+          (ensures distinct_assoc_fst (apply_log s l) /\ length (apply_log s l) = length s + length l)
           (decreases length l) =
   match length l with
   |0 -> ()
   |_ -> mem_cons (head l) (tail l);
        distinct_invert_append (create 1 (head l)) (tail l);
        do_is_unique s (head l); 
-       lemma_append_count_assoc_fst (create 1 (fst (head l), snd (head l))) s; 
-       lem_foldl1 (do s (head l)) (tail l)
+       lemma_append_count_assoc_fst (create 1 (fst (head l), snd (head l))) s;
+       lem_foldl_uni (do s (head l)) (tail l)
 #pop-options
 
 let valid_is_unique (s:st0) 
   : Lemma (requires distinct_ops (ops_of s) /\ v_of s == apply_log init_st (ops_of s))
-          (ensures unique_st (v_of s) /\ length (v_of s) = length (ops_of s)) =
-  lem_foldl1 init_st (ops_of s)
-
-let lem_diff_s (s1 lca:concrete_st)
-  : Lemma (requires is_suffix_s lca s1 /\ unique_st s1)
-          (ensures (forall id. (mem_id_s id s1 /\ not (mem_id_s id lca)) <==> (mem_id_s id (diff_s s1 lca))) /\
-                   unique_st (diff_s s1 lca)) =
-  lemma_append_count_assoc_fst (diff_s s1 lca) lca
+          (ensures distinct_assoc_fst (v_of s) /\ length (v_of s) = length (ops_of s)) =
+  lem_foldl_uni init_st (ops_of s)
 
 #push-options "--z3rlimit 50"
-let rec lem_not_id (a b:concrete_st) (al bl:log)
-  : Lemma (requires (forall id. mem_id_s id a <==> mem_id id al) /\
-                    (forall id. mem_id_s id b <==> mem_id id bl) /\
-                    (forall id. mem_id id al ==> not (mem_id id bl)) /\
-                    distinct_ops al /\ distinct_ops bl /\
-                    unique_st a /\ unique_st b /\
-                    length al = length a /\
-                    length bl = length b)
-          (ensures (forall id. mem_id_s id a ==> not (mem_id_s id b)))
-          (decreases %[length al]) =
-  match length al with
-  |0 -> ()
-  |_ -> remove_is_uni a (fst (head al));
-       remove_is_uni al (fst (head al));
-       let ras = (remove_id a (fst (head al))) in
-       let ra = (remove_id al (fst (head al))) in
-       lem_not_id ras b ra bl
-
 let merge_is_comm (lca s1 s2:st)
   : Lemma (requires consistent_branches lca s1 s2 /\
                     (exists l1 l2. apply_log (v_of lca) l1 == (v_of s1) /\ apply_log (v_of lca) l2 == (v_of s2)))
@@ -186,33 +138,33 @@ let merge_is_comm (lca s1 s2:st)
   split_prefix init_st (ops_of lca) (ops_of s2);
   lem_foldl (v_of lca) (diff (ops_of s1) (ops_of lca));
   lem_foldl (v_of lca) (diff (ops_of s2) (ops_of lca));
-  let la = diff_s (v_of s1) (v_of lca) in
-  let lb = diff_s (v_of s2) (v_of lca) in
+  let la = diff_suf (v_of s1) (v_of lca) in
+  let lb = diff_suf (v_of s2) (v_of lca) in
   let u1 = union_s la lb in 
   let u2 = union_s lb la in
   valid_is_unique lca;
   valid_is_unique s1;
   valid_is_unique s2;
-  lem_diff_s (v_of s1) (v_of lca);
-  lem_diff_s (v_of s2) (v_of lca);
-  assert (forall id. mem_id_s id (v_of lca) <==> mem_id id (ops_of lca));
-  assert (forall id. mem_id_s id (v_of s1) <==> mem_id_s id (v_of lca) \/ mem_id id (diff (ops_of s1) (ops_of lca)));
-  assert (forall id. mem_id_s id (v_of s2) <==> mem_id_s id (v_of lca) \/ mem_id id (diff (ops_of s2) (ops_of lca)));
-  assert (forall id. mem_id_s id (v_of s1) <==> mem_id_s id (v_of lca) \/ mem_id_s id (diff_s (v_of s1) (v_of lca)));
-  assert (forall id. mem_id_s id (v_of s2) <==> mem_id_s id (v_of lca) \/ mem_id_s id (diff_s (v_of s2) (v_of lca)));
-  assert (forall id. (mem_id_s id (v_of s1) /\ not (mem_id_s id (v_of lca))) <==> (mem_id_s id la)); 
-  assert (forall id. (mem_id_s id (v_of s2) /\ not (mem_id_s id (v_of lca))) <==> (mem_id_s id lb)); 
+  lem_diff_suf_uni (v_of s1) (v_of lca);
+  lem_diff_suf_uni (v_of s2) (v_of lca); 
+  assert (forall id. mem_assoc_fst id (v_of lca) <==> mem_id id (ops_of lca));
+  assert (forall id. mem_assoc_fst id (v_of s1) <==> mem_assoc_fst id (v_of lca) \/ mem_id id (diff (ops_of s1) (ops_of lca)));
+  assert (forall id. mem_assoc_fst id (v_of s2) <==> mem_assoc_fst id (v_of lca) \/ mem_id id (diff (ops_of s2) (ops_of lca)));
+  assert (forall id. mem_assoc_fst id (v_of s1) <==> mem_assoc_fst id (v_of lca) \/ mem_assoc_fst id (diff_suf (v_of s1) (v_of lca)));
+  assert (forall id. mem_assoc_fst id (v_of s2) <==> mem_assoc_fst id (v_of lca) \/ mem_assoc_fst id (diff_suf (v_of s2) (v_of lca)));
+  assert (forall id. (mem_assoc_fst id (v_of s1) /\ not (mem_assoc_fst id (v_of lca))) <==> (mem_assoc_fst id la)); 
+  assert (forall id. (mem_assoc_fst id (v_of s2) /\ not (mem_assoc_fst id (v_of lca))) <==> (mem_assoc_fst id lb));
   lem_diff (ops_of s1) (ops_of lca);
   lem_diff (ops_of s2) (ops_of lca);
-  lem_foldl1 (v_of lca) (diff (ops_of s1) (ops_of lca));
-  lem_foldl1 (v_of lca) (diff (ops_of s2) (ops_of lca));
-  assert (forall id. mem_id_s id la <==> mem_id id (diff (ops_of s1) (ops_of lca)));
-  assert (forall id. mem_id_s id lb <==> mem_id id (diff (ops_of s2) (ops_of lca)));
-  assert (forall id. mem_id_s id la <==> mem_id id (diff (ops_of s1) (ops_of lca))); 
-  assert (forall id. mem_id_s id lb <==> mem_id id (diff (ops_of s2) (ops_of lca))); 
-  assert (forall id. mem_id id (diff (ops_of s1) (ops_of lca)) ==> not (mem_id id (diff (ops_of s2) (ops_of lca)))); 
-  lem_not_id la lb (diff (ops_of s1) (ops_of lca)) (diff (ops_of s2) (ops_of lca)); 
-  assert (forall id. mem_id_s id la ==> not (mem_id_s id lb)); 
+  lem_foldl_uni (v_of lca) (diff (ops_of s1) (ops_of lca));
+  lem_foldl_uni (v_of lca) (diff (ops_of s2) (ops_of lca));
+  assert (forall id. mem_assoc_fst id la <==> mem_id id (diff (ops_of s1) (ops_of lca)));
+  assert (forall id. mem_assoc_fst id lb <==> mem_id id (diff (ops_of s2) (ops_of lca)));
+  assert (forall id. mem_assoc_fst id la <==> mem_id id (diff (ops_of s1) (ops_of lca))); 
+  assert (forall id. mem_assoc_fst id lb <==> mem_id id (diff (ops_of s2) (ops_of lca))); 
+  assert (forall id. mem_id id (diff (ops_of s1) (ops_of lca)) ==> not (mem_id id (diff (ops_of s2) (ops_of lca))));
+  lem_not_mem_id la lb (diff (ops_of s1) (ops_of lca)) (diff (ops_of s2) (ops_of lca)); 
+  assert (forall id. mem_assoc_fst id la ==> not (mem_assoc_fst id lb)); 
   lem_union_comm la lb;
   assert (union_s la lb == union_s lb la);
   ()
@@ -226,7 +178,6 @@ let linearizable_s1_0''_base_base (lca s1 s2':st) (last2:op_t)
         
           (ensures eq (do (v_of s2') last2) (concrete_merge (v_of lca) (v_of s1) (do (v_of s2') last2))) = ()
 
-#push-options "--z3rlimit 50"
 let linearizable_s1_0''_base_ind (lca s1 s2':st) (last2:op_t)
   : Lemma (requires consistent_branches lca s1 s2' /\
                     is_prefix (ops_of lca) (snoc (ops_of s2') last2) /\
@@ -243,7 +194,6 @@ let linearizable_s1_0''_base_ind (lca s1 s2':st) (last2:op_t)
                     eq (do (v_of s2'') last2) (concrete_merge (v_of l') (v_of s1') (do (v_of s2'') last2))))
 
           (ensures eq (do (v_of s2') last2) (concrete_merge (v_of lca) (v_of s1) (do (v_of s2') last2))) = ()
-#pop-options
 
 let linearizable_s1_0''_ind (lca s1 s2':st) (last2:op_t)
   : Lemma (requires consistent_branches_s2_gt0 lca s1 s2' /\
@@ -267,7 +217,6 @@ let linearizable_s1_0_s2_0_base (lca s1 s2:st)
         
           (ensures eq (v_of lca) (concrete_merge (v_of lca) (v_of s1) (v_of s2))) = ()
           
-#push-options "--z3rlimit 50"
 let linearizable_gt0_base_last1 (lca s1 s2:st) (last1 last2:op_t)
   : Lemma (requires consistent_branches lca s1 s2 /\
                     ops_of s1 = ops_of lca /\ ops_of s2 = ops_of lca /\
@@ -324,19 +273,6 @@ let linearizable_gt0_base (lca s1 s2:st) (last1 last2:op_t)
     linearizable_gt0_base_last1 lca s1 s2 last1 last2
   else linearizable_gt0_base_last2 lca s1 s2 last1 last2
 
-let lem_diff_s1 (s1 l:concrete_st)
-  : Lemma (requires is_suffix_s l s1)
-          (ensures (Seq.length s1 > Seq.length l ==> (head s1 == head (diff_s s1 l) /\ Seq.length (diff_s s1 l) > 0) /\
-                     (let h1 = head s1 in
-                      let hd = head (diff_s s1 l) in
-                      h1 = hd) /\
-                     (let s1' = tail s1 in 
-                       is_suffix_s l s1' /\
-                       diff_s s1' l == tail (diff_s s1 l))))
-  = let s = fst (split s1 (length s1 - length l)) in
-    lemma_split s1 (length s1 - length l);
-    lemma_mem_append s l
-
 let lem_unionb (a b:concrete_st)
   : Lemma (requires length a > 0 /\ length b > 0 /\
                     lt (fst (head a)) (fst (head b)))
@@ -364,16 +300,16 @@ let linearizable_gt0_ind_c2 (lca s1 s2:st) (last1 last2:op_t)
                       (concrete_merge (v_of lca) (do (v_of s1) last1) (do (v_of s2) last2)))] = 
   let s1v = do (v_of s1) last1 in
   let s2v = do (v_of s2) last2 in
-  let da = (diff_s s1v (v_of lca)) in
-  let db = (diff_s s2v (v_of lca)) in
-  let db' = (diff_s (v_of s2) (v_of lca)) in
-  let da' = (diff_s (v_of s1) (v_of lca)) in
+  let da = (diff_suf s1v (v_of lca)) in
+  let db = (diff_suf s2v (v_of lca)) in
+  let db' = (diff_suf (v_of s2) (v_of lca)) in
+  let da' = (diff_suf (v_of s1) (v_of lca)) in
   let l1 = (fst last1, snd last1) in
   let l2 = (fst last2, snd last2) in 
   lemma_tl l2 (v_of s2); 
-  lem_diff_s1 s2v (v_of lca); 
-  lemma_tl l1 (v_of s1); 
-  lem_diff_s1 s1v (v_of lca);
+  lem_diff_suf s2v (v_of lca); 
+  lemma_tl l1 (v_of s1);
+  lem_diff_suf s1v (v_of lca);  
   assert (lt (fst last1) (fst (last2)));
   assert (lt (fst (head da)) (fst (head db))); 
   lem_unionb da db;
@@ -396,16 +332,16 @@ let linearizable_gt0_ind1_c1 (lca s1 s2:st) (last1 last2:op_t)
                       (concrete_merge (v_of lca) (do (v_of s1) last1) (do (v_of s2) last2)))] = 
   let s1v = do (v_of s1) last1 in
   let s2v = do (v_of s2) last2 in
-  let da = (diff_s s1v (v_of lca)) in
-  let db = (diff_s s2v (v_of lca)) in
-  let da' = (diff_s (v_of s1) (v_of lca)) in
-  let db' = (diff_s (v_of s2) (v_of lca)) in
+  let da = (diff_suf s1v (v_of lca)) in
+  let db = (diff_suf s2v (v_of lca)) in
+  let da' = (diff_suf (v_of s1) (v_of lca)) in
+  let db' = (diff_suf (v_of s2) (v_of lca)) in
   let l1 = (fst last1, snd last1) in
   let l2 = (fst last2, snd last2) in
   lemma_tl l1 (v_of s1);
-  lem_diff_s1 s1v (v_of lca);
+  lem_diff_suf s1v (v_of lca);
   lemma_tl l2 (v_of s2);
-  lem_diff_s1 s2v (v_of lca);
+  lem_diff_suf s2v (v_of lca);
   assert (lt (fst last2) (fst (last1)));
   assert (lt (fst (head db)) (fst (head da)));
   lem_uniona da db; 
